rename Key type to OwnedKey

messageInvariantPrototypes/shardedKv/types.dfy
@@ -4,10 +4,10 @@ module Types {
   import opened UtilitiesLibrary
 
   type HostId = nat
-  type Key = int
+  type OwnedKey = int
   datatype Entry = Entry(live: bool, version: nat)
 
-  datatype Message = Reconf(src: nat, dst: nat, key: Key, version: nat) 
+  datatype Message = Reconf(src: nat, dst: nat, key: OwnedKey, version: nat) 
 
   datatype MessageOps = MessageOps(recv:Option<Message>, send:Option<Message>)
 } // end module Types
